WIP: Preliminary definitions and lemmas

Compilation.thy
@@ -4,7 +4,7 @@ begin
 
 text \<open>This formalisation follows the pen-and-paper compilation defined by Gigante, et al.\<close>
 
-datatype ('proposition, 'action, 'snap_action) state =
+datatype ('proposition, 'action, 'snap_action) location =
   Init 
   | Goal
   | Main
@@ -27,7 +27,7 @@ datatype ('proposition, 'action) clock =
 datatype alpha = Unit
 
 context temp_planning_problem
-begin
+begin                 
 
 definition prop_numbers ("p\<^sub>_" 65) where "prop_numbers \<equiv> p"
 
@@ -40,47 +40,49 @@ definition "M = card actions"
 definition "true_const \<equiv> GE Stop 0"
 
 text \<open>Preventing time from passing in any location other than the main location.\<close>
-fun invs::"(('proposition, 'action) clock, 't, ('proposition, 'action, 'snap_action) state) invassn" where
+fun invs::"(('proposition, 'action) clock, 'time, ('proposition, 'action, 'snap_action) location) invassn" where
   "invs Main  = GE Stop 0"
 | "invs _     = EQ Stop 0"
 
+abbreviation "prop_list S \<equiv> sorted_key_list_of_set (inv p) S"
+
 text \<open>The transition from the initial location \<open>l\<^sub>I\<close> to the main location \<open>l\<^sub>\<delta>\<close>\<close>
 definition init_pos::"'proposition list" where
-"init_pos \<equiv> sorted_key_list_of_set (inv p) init"
+"init_pos \<equiv> prop_list init"
 
-definition init_asmt::"(('proposition, 'action) clock, 't) clkassn list" where
+definition init_asmt::"(('proposition, 'action) clock, 'time) clkassn list" where
 "init_asmt \<equiv> map (\<lambda>x. (PropClock x, 1)) init_pos"
 
-definition initial_transition::"(alpha, ('proposition, 'action) clock, 't, ('proposition, 'action, 'snap_action) state) transition" where
+definition initial_transition::"(alpha, ('proposition, 'action) clock, 'time, ('proposition, 'action, 'snap_action) location) transition" where
 "initial_transition \<equiv> (Init, true_const, Unit, init_asmt, Main)"
 
-text \<open>The transition from the main location \<open>l\<^sub>\<delta>\<close> to the \<open>0\<^sup>t\<^sup>h\<close> location of the state decoding path \<open>s\<^sub>0\<close>.\<close>
-definition main_to_decoding::"(alpha, ('proposition, 'action) clock, 't, ('proposition, 'action, 'snap_action) state) transition" where
+text \<open>The transition from the main location \<open>l\<^sub>\<delta>\<close> to the \<open>0\<^sup>t\<^sup>h\<close> location of the location decoding path \<open>s\<^sub>0\<close>.\<close>
+definition main_to_decoding::"(alpha, ('proposition, 'action) clock, 'time, ('proposition, 'action, 'snap_action) location) transition" where
 "main_to_decoding \<equiv> (Main, true_const, Unit, [(Stop, 0)], PropDecoding (p 0))"
 
 subsubsection \<open>State decoding\<close>
 
 text \<open>The transitions between the decoding locations for the propositional clocks \<open>cp\<^sub>i\<close>\<close>
-definition prop_decoding::"(alpha, ('proposition, 'action) clock, 't, ('proposition, 'action, 'snap_action) state) transition set" where
+definition prop_decoding::"(alpha, ('proposition, 'action) clock, 'time, ('proposition, 'action, 'snap_action) location) transition set" where
 "prop_decoding \<equiv> {(PropDecoding (p n), CEQ (PropClock (p n)) Delta 1, Unit, [(PropClock (p n), 1)], PropDecoding (p (n + 1))) | n. n < N}
   \<union> {(PropDecoding (p n), CEQ (PropClock (p n)) Delta 0, Unit, [(PropClock (p n), 0)], PropDecoding (p (n + 1))) | n. n < N}"
 
 text \<open>A transition from the decoding locations for propositional clocks to the decoding locations for
 the execution clocks\<close>
-definition prop_decoding_to_exec_decoding::"(alpha, ('proposition, 'action) clock, 't, ('proposition, 'action, 'snap_action) state) transition" where
+definition prop_decoding_to_exec_decoding::"(alpha, ('proposition, 'action) clock, 'time, ('proposition, 'action, 'snap_action) location) transition" where
 "prop_decoding_to_exec_decoding \<equiv> (PropDecoding (p N), true_const, Unit, [], ExecDecoding (act 0))"
 
 text \<open>The transitions between the decoding locations for the execution clocks \<open>cr\<^sub>a\<close>\<close>
-definition exec_decoding::"(alpha, ('proposition, 'action) clock, 't, ('proposition, 'action, 'snap_action) state) transition set" where
+definition exec_decoding::"(alpha, ('proposition, 'action) clock, 'time, ('proposition, 'action, 'snap_action) location) transition set" where
 "exec_decoding \<equiv> {(ExecDecoding (act m), CEQ (Running (act m)) Delta 1, Unit, [(Running (act m), 1)], ExecDecoding (act (m + 1))) | m. m < M}
   \<union> {(ExecDecoding (act m), CEQ (Running (act m)) Delta 0, Unit, [(Running (act m), 0)], ExecDecoding (act (m + 1))) | m. m < M}"
 
 text \<open>The transition from the execution decoding locations to the decision-making locations\<close>
-definition exec_decoding_to_decision_making::"(alpha, ('proposition, 'action) clock, 't, ('proposition, 'action, 'snap_action) state) transition" where
+definition exec_decoding_to_decision_making::"(alpha, ('proposition, 'action) clock, 'time, ('proposition, 'action, 'snap_action) location) transition" where
 "exec_decoding_to_decision_making \<equiv> (ExecDecoding (act M), true_const, Unit, [], Decision (at_start (act 0)))"
 
 subsubsection \<open>Decision-making\<close>
-definition AND_ALL::"(('proposition, 'action) clock, 't) dconstraint list \<Rightarrow> (('proposition, 'action) clock, 't) dconstraint" where
+definition AND_ALL::"(('proposition, 'action) clock, 'time) dconstraint list \<Rightarrow> (('proposition, 'action) clock, 'time) dconstraint" where
 "AND_ALL xs = fold AND xs (true_const)"
 
 text \<open>Numbering for snap_actions. This is hard to work with.\<close>
@@ -350,33 +352,33 @@ text \<open>This is easier to work with.\<close>
 definition interfering_at_start::"'snap_action \<Rightarrow> nat list" where
 "interfering_at_start a = sorted_list_of_set {n. at_start (act n) \<noteq> a \<and> mutex_snap_action a (at_start (act n))}"
 
-definition start_constraints::"'snap_action \<Rightarrow> (('proposition, 'action) clock, 't) dconstraint list" where
+definition start_constraints::"'snap_action \<Rightarrow> (('proposition, 'action) clock, 'time) dconstraint list" where
 "start_constraints a = map (\<lambda>b. GT (Start (act b)) \<epsilon>) (interfering_at_start a)"
 
 definition interfering_at_end::"'snap_action \<Rightarrow> nat list" where
 "interfering_at_end a = sorted_list_of_set {n. at_end (act n) \<noteq> a \<and> mutex_snap_action a (at_end (act n))}"
 
-definition end_constraints::"'snap_action \<Rightarrow> (('proposition, 'action) clock, 't) dconstraint list" where
+definition end_constraints::"'snap_action \<Rightarrow> (('proposition, 'action) clock, 'time) dconstraint list" where
 "end_constraints a = map (\<lambda>b. GT (End (act b)) \<epsilon>) (interfering_at_end a)"
 
-definition sep::"'snap_action \<Rightarrow> (('proposition, 'action) clock, 't) dconstraint" where
+definition sep::"'snap_action \<Rightarrow> (('proposition, 'action) clock, 'time) dconstraint" where
 "sep a \<equiv> AND_ALL (start_constraints a @ end_constraints a)"
 
 text \<open>The clock constraints for the precondition\<close>
 definition pre_clocks::"'snap_action \<Rightarrow> ('proposition, 'action) clock list" where
-"pre_clocks a \<equiv> map PropClock (sorted_key_list_of_set (inv p) (pre a))"
+"pre_clocks a \<equiv> map PropClock (prop_list (pre a))"
 
-definition pre_constraint::"'snap_action \<Rightarrow> (('proposition, 'action) clock, 't) dconstraint" where
+definition pre_constraint::"'snap_action \<Rightarrow> (('proposition, 'action) clock, 'time) dconstraint" where
 "pre_constraint a \<equiv> AND_ALL (map (\<lambda>c. EQ c 1) (pre_clocks a))"
 
 text \<open>The guard constraints\<close>
-definition guard::"'snap_action \<Rightarrow> (('proposition, 'action) clock, 't) dconstraint" where
+definition guard::"'snap_action \<Rightarrow> (('proposition, 'action) clock, 'time) dconstraint" where
 "guard a \<equiv> AND (sep a) (pre_constraint a)"
 
-definition guard_at_start::"'action \<Rightarrow> (('proposition, 'action) clock, 't::time) dconstraint" where
+definition guard_at_start::"'action \<Rightarrow> (('proposition, 'action) clock, 'time::time) dconstraint" where
 "guard_at_start a \<equiv> AND (guard (at_start a)) (EQ (Running a) 0)"
 
-definition guard_at_end::"'action \<Rightarrow> (('proposition, 'action) clock, 't::time) dconstraint" where
+definition guard_at_end::"'action \<Rightarrow> (('proposition, 'action) clock, 'time::time) dconstraint" where
 "guard_at_end a \<equiv> 
   let l = case (lower a) of 
     (lower_bound.GT t) \<Rightarrow> GT (Start a) t
@@ -387,34 +389,34 @@ definition guard_at_end::"'action \<Rightarrow> (('proposition, 'action) clock, 
   in
 AND (AND (guard (at_end a)) (EQ (Running a) 1)) (AND l u)"
 
-definition decision_making::"(alpha, ('proposition, 'action) clock, 't, ('proposition, 'action, 'snap_action) state) transition set" where
+definition decision_making::"(alpha, ('proposition, 'action) clock, 'time, ('proposition, 'action, 'snap_action) location) transition set" where
 "decision_making \<equiv> 
   {(Decision (at_start (act m)), guard (at_start (act m)), Unit, [(ExecStart (act m), 1)], Decision (at_end (act m))) | m. m < M}
   \<union> {(Decision (at_start (act m)), true_const, Unit, [(ExecStart (act m), 0)], Decision (at_end (act m))) | m. m < M}
   \<union> {(Decision (at_end (act m)), guard (at_end (act m)), Unit, [(ExecEnd (act m), 1)], Decision (at_start (act (Suc m)))) | m. Suc m < M}
   \<union> {(Decision (at_end (act m)), true_const, Unit, [(ExecEnd (act m), 0)], Decision (at_start (act (Suc m)))) | m. Suc m < M}"
 
-definition dm_to_exec::"(alpha, ('proposition, 'action) clock, 't, ('proposition, 'action, 'snap_action) state) transition" where
+definition dm_to_exec::"(alpha, ('proposition, 'action) clock, 'time, ('proposition, 'action, 'snap_action) location) transition" where
 "dm_to_exec \<equiv> (Decision (at_end (act M)), true_const, Unit, [], Execution (at_start (act 0)))"
 
 subsubsection \<open>Execution\<close>
 
-definition add_effects::"'snap_action \<Rightarrow> (('proposition, 'action) clock, 't) clkassn list" where
-"add_effects s \<equiv> map (\<lambda>p. (PropClock p, 1)) (sorted_key_list_of_set (inv p) (adds s))"
+definition add_effects::"'snap_action \<Rightarrow> (('proposition, 'action) clock, 'time) clkassn list" where
+"add_effects s \<equiv> map (\<lambda>p. (PropClock p, 1)) (prop_list (adds s))"
 
-definition del_effects::"'snap_action  \<Rightarrow> (('proposition, 'action) clock, 't) clkassn list" where
-"del_effects s \<equiv> map (\<lambda>p. (PropClock p, 1)) (sorted_key_list_of_set (inv p) ((dels s) - (adds s)))"
+definition del_effects::"'snap_action  \<Rightarrow> (('proposition, 'action) clock, 'time) clkassn list" where
+"del_effects s \<equiv> map (\<lambda>p. (PropClock p, 1)) (prop_list ((dels s) - (adds s)))"
 
-definition effects::"'snap_action \<Rightarrow> (('proposition, 'action) clock, 't) clkassn list" where
+definition effects::"'snap_action \<Rightarrow> (('proposition, 'action) clock, 'time) clkassn list" where
 "effects s \<equiv> del_effects s @ add_effects s"
 
-definition at_start_effects::"'action \<Rightarrow> (('proposition, 'action) clock, 't) clkassn list" where
+definition at_start_effects::"'action \<Rightarrow> (('proposition, 'action) clock, 'time) clkassn list" where
 "at_start_effects a \<equiv> (Running a, 1) # (ExecStart a, 0) # effects (at_start a)"
 
-definition at_end_effects::"'action \<Rightarrow> (('proposition, 'action) clock, 't) clkassn list" where
+definition at_end_effects::"'action \<Rightarrow> (('proposition, 'action) clock, 'time) clkassn list" where
 "at_end_effects a \<equiv> (Running a, 0) # (ExecEnd a, 0) # effects (at_start a)"
 
-definition execution::"(alpha, ('proposition, 'action) clock, 't, ('proposition, 'action, 'snap_action) state) transition set" where
+definition execution::"(alpha, ('proposition, 'action) clock, 'time, ('proposition, 'action, 'snap_action) location) transition set" where
 "execution \<equiv> 
   {(Execution (at_start (act m)), EQ (ExecStart (act m)) 1, Unit, at_start_effects (act m), Execution (at_end (act m))) | m. m < M}
   \<union> {(Execution (at_start (act m)), true_const, Unit, [], Execution (at_end (act m))) | m. m < M}
@@ -423,36 +425,176 @@ definition execution::"(alpha, ('proposition, 'action) clock, 't, ('proposition,
 
 
 subsubsection \<open>Over-all conditions\<close>
-definition over_all_clocks::"'action \<Rightarrow> ('proposition, 'action) clock list" where
-"over_all_clocks a \<equiv> map PropClock (sorted_key_list_of_set (inv p) (over_all a))"
+abbreviation "action_list \<equiv> map act (sorted_list_of_set {m. m < M})"
 
-definition action_over_all::"'action \<Rightarrow> (('proposition, 'action) clock, 't) dconstraint" where
+definition over_all_clocks::"'action \<Rightarrow> ('proposition, 'action) clock list" where
+"over_all_clocks a \<equiv> map PropClock (prop_list (over_all a))"
+
+definition action_over_all::"'action \<Rightarrow> (('proposition, 'action) clock, 'time) dconstraint" where
 "action_over_all a \<equiv> AND_ALL (map (\<lambda>c. CLE (Running a) c 0) (over_all_clocks a))"
 
-definition over_all_conds::"(('proposition, 'action) clock, 't) dconstraint" where
-"over_all_conds \<equiv> AND_ALL (map (\<lambda>m. action_over_all (act m)) (sorted_list_of_set {m. m < M}))"
+definition over_all_conds::"(('proposition, 'action) clock, 'time) dconstraint" where
+"over_all_conds \<equiv> AND_ALL (map action_over_all action_list)"
 
-definition exec_to_main::"(alpha, ('proposition, 'action) clock, 't, ('proposition, 'action, 'snap_action) state) transition" where
+definition exec_to_main::"(alpha, ('proposition, 'action) clock, 'time, ('proposition, 'action, 'snap_action) location) transition" where
 "exec_to_main \<equiv> (Execution (at_end (act M)), over_all_conds, Unit, [(Delta, 0)], Main)"
 
 subsubsection \<open>The goal\<close>
-definition none_running::"(('proposition, 'action) clock, 't) dconstraint" where
-"none_running \<equiv> AND_ALL (map (\<lambda>m. EQ (Running (act m)) 0) (sorted_list_of_set {m. m < M}))"
+definition none_running::"(('proposition, 'action) clock, 'time) dconstraint" where
+"none_running \<equiv> AND_ALL (map (\<lambda>a. EQ (Running a) 0) action_list)"
 
-definition goal_satisfied::"(('proposition, 'action) clock, 't) dconstraint" where
-"goal_satisfied \<equiv> AND_ALL (map (\<lambda>p. EQ (PropClock p) 1) (sorted_key_list_of_set (inv p) goal))"
+definition goal_satisfied::"(('proposition, 'action) clock, 'time) dconstraint" where
+"goal_satisfied \<equiv> AND_ALL (map (\<lambda>p. EQ (PropClock p) 1) (prop_list goal))"
 
-definition goal_constraint::"(('proposition, 'action) clock, 't) dconstraint" where
+definition goal_constraint::"(('proposition, 'action) clock, 'time) dconstraint" where
 "goal_constraint \<equiv> AND none_running goal_satisfied"
 
-definition goal_trans::"(alpha, ('proposition, 'action) clock, 't, ('proposition, 'action, 'snap_action) state) transition" where
+definition goal_trans::"(alpha, ('proposition, 'action) clock, 'time, ('proposition, 'action, 'snap_action) location) transition" where
 "goal_trans \<equiv> (ExecDecoding (act M), goal_constraint, Unit, [], Goal)"
 
 subsubsection \<open>The automaton\<close>
-definition plan_automaton::"(alpha, ('proposition, 'action) clock, 't, ('proposition, 'action, 'snap_action) state) ta" where
-"plan_automaton \<equiv> ({initial_transition} \<union> {main_to_decoding} \<union> prop_decoding 
+definition prob_automaton::"(alpha, ('proposition, 'action) clock, 'time, ('proposition, 'action, 'snap_action) location) ta" ("\<T>") where
+"prob_automaton \<equiv> ({initial_transition} \<union> {main_to_decoding} \<union> prop_decoding 
   \<union> {prop_decoding_to_exec_decoding} \<union> exec_decoding \<union> {exec_decoding_to_decision_making}
   \<union> decision_making \<union> {dm_to_exec} \<union> execution \<union> {exec_to_main} \<union> {goal_trans}, invs)"
+end
+
+context temporal_plan
+begin
+
+subsection \<open>Definitions\<close>
+subsubsection \<open>Proposition and execution model\<close>
+definition prop_model::"(('proposition, 'action) clock, 'time) cval \<Rightarrow> 'proposition state \<Rightarrow> bool" where
+"prop_model W Q \<equiv> \<forall>p. (W (PropClock p) = 1 \<longleftrightarrow> p \<in> Q) \<and> (W (PropClock p) = 0 \<longleftrightarrow> p \<notin> Q)"
+
+definition delta_prop_model::"(('proposition, 'action) clock, 'time) cval \<Rightarrow> 'proposition state \<Rightarrow> bool" where
+"delta_prop_model W Q \<equiv> \<forall>p. ((W (PropClock p)) - (W Delta) = 1 \<longleftrightarrow> p \<in> Q) \<and> ((W (PropClock p)) - (W Delta) = 0 \<longleftrightarrow> p \<notin> Q)"
+
+type_synonym 'a exec_state = "'a set"
+
+definition exec_model::"(('proposition, 'action) clock, 'time) cval \<Rightarrow> 'action exec_state \<Rightarrow> bool" where
+"exec_model W E \<equiv> \<forall>a \<in> actions. (W (Running a) = 1 \<longleftrightarrow> a \<in> E) \<and> (W (Running a) = 0 \<longleftrightarrow> a \<notin> E)"
+
+definition delta_exec_model::"(('proposition, 'action) clock, 'time) cval \<Rightarrow> 'action exec_state \<Rightarrow> bool" where
+"delta_exec_model W E \<equiv> \<forall>a \<in> actions. ((W (Running a)) - (W Delta) = 1 \<longleftrightarrow> a \<in> E) \<and> ((W (Running a)) - (W Delta) = 0 \<longleftrightarrow> a \<notin> E)"
+
+definition partial_exec_model::"(('proposition, 'action) clock, 'time) cval \<Rightarrow> 'action exec_state \<Rightarrow> bool" where
+"partial_exec_model W E \<equiv> \<forall>m < M. (W (Running (act m)) = 1 \<longleftrightarrow> (act m) \<in> E) \<and> (W (Running (act m)) = 0 \<longleftrightarrow> (act m) \<notin> E)"
+
+
+subsubsection \<open>Execution time\<close>
+definition argmax::"('ty::linordered_ab_group_add \<Rightarrow> bool) \<Rightarrow> 'ty" where
+"argmax P \<equiv> if (\<exists>x. P x) then (Greatest P) else 0"
+
+abbreviation "B" where "B \<equiv> happ_at plan_happ_seq"
+
+definition last_snap_exec::"'snap_action \<Rightarrow> 'time \<Rightarrow> 'time" where
+"last_snap_exec a t = argmax (\<lambda>t'. t' < t \<and> a \<in> B t')"
+
+definition exec_time::"'snap_action \<Rightarrow> 'time \<Rightarrow> 'time" where
+"exec_time a t = (let t' = last_snap_exec a t in t - t')"
+
+definition last_snap_exec'::"'snap_action \<Rightarrow> 'time \<Rightarrow> 'time" where
+"last_snap_exec' a t = argmax (\<lambda>t'. t' \<le> t \<and> a \<in> B t')"
+
+definition exec_time'::"'snap_action \<Rightarrow> 'time \<Rightarrow> 'time" where
+"exec_time' a t = (let t' = last_snap_exec' a t in t - t')"
+
+
+
+lemma a_not_in_b_last_unchanged: "a \<notin> B t \<Longrightarrow> last_snap_exec' a t = last_snap_exec a t"
+proof -
+  assume "a \<notin> B t"
+  have 1: "(GREATEST t'. t' < t \<and> a \<in> B t') = (GREATEST t'. t' \<le> t \<and> a \<in> B t')"
+    if defined: "\<exists>x\<le>t. a \<in> B x"
+  proof (rule classical)
+    assume "(GREATEST t'. t' < t \<and> a \<in> B t') \<noteq> (GREATEST t'. t' \<le> t \<and> a \<in> B t')"
+    then have "\<exists>t'. t' \<le> t \<and> \<not>(t' < t) \<and> a \<in> B t'"
+      using defined
+      by (meson nless_le)
+    then have "a \<in> B t" by auto
+    with \<open>a \<notin> B t\<close>
+    have "False" by simp
+    thus "(GREATEST t'. t' < t \<and> a \<in> B t') = (GREATEST t'. t' \<le> t \<and> a \<in> B t')"
+      by blast
+  qed
+  from \<open>a \<notin> B t\<close>
+  have "(\<exists>x<t. a \<in> B x) = (\<exists>x\<le>t. a \<in> B x)"
+    using nless_le by auto
+  with \<open>a \<notin> B t\<close> 1
+  have "argmax (\<lambda>t'. t' < t \<and> a \<in> B t') = argmax (\<lambda>t'. t' \<le> t \<and> a \<in> B t')"
+    unfolding argmax_def using 1 by argo
+  thus "last_snap_exec' a t = last_snap_exec a t"
+    using last_snap_exec_def last_snap_exec'_def by simp
+qed
+
+lemma a_in_b_last_now: "a \<in> B t \<Longrightarrow> last_snap_exec' a t = t"
+  unfolding last_snap_exec'_def
+  argmax_def
+  by (auto intro: Greatest_equality)
+
+
+subsubsection \<open>Restricting snap action sets by an upper limit on the index\<close>
+
+definition limited_snap_action_set::"'snap_action set \<Rightarrow> nat \<Rightarrow> 'snap_action set" where
+"limited_snap_action_set S m = 
+  {at_start (act n) | n. n < m \<and> at_start (act n) \<in> S} 
+  \<union> {at_end (act n) | n. n < m \<and> at_end (act n) \<in> S}"
+
+lemma limit_M_eq_orig: "S \<subseteq> snap_actions \<Longrightarrow> limited_snap_action_set S M = S"
+proof (rule equalityI; rule subsetI)
+  fix x
+  assume S: "S \<subseteq> snap_actions" 
+     and x: "x \<in> limited_snap_action_set S M"
+  from x obtain n where
+    "x = at_start (act n) \<and> at_start (act n) \<in> S 
+    \<or> x = at_end (act n) \<and> at_end (act n) \<in> S"
+    unfolding limited_snap_action_set_def by blast         
+  then show "x \<in> S" by blast
+next 
+  fix x
+  assume S: "S \<subseteq> snap_actions" 
+     and x: "x \<in> S"
+  hence "x \<in> at_start ` actions \<or> x \<in> at_end ` actions" 
+    unfolding snap_actions_def by blast
+  hence "\<exists>m. m < (card actions) \<and> (x = at_start (act m) \<or> x = at_end (act m))" 
+    using act_img_action by force
+  with x
+  show "x \<in> limited_snap_action_set S M" unfolding M_def limited_snap_action_set_def
+    by blast
+qed
+
+abbreviation B_lim::"'time \<Rightarrow> nat \<Rightarrow> 'snap_action set" where
+"B_lim t m \<equiv> limited_snap_action_set (B t) m"
+
+definition partial_exec_time_update::"'snap_action \<Rightarrow> 'time \<Rightarrow> nat \<Rightarrow> 'time" where
+"partial_exec_time_update a t m \<equiv> if (a \<in> B_lim t m) then 0 else exec_time a t"
+
+lemma B_lim_M_eq_B: "B_lim t M = B t" 
+proof (rule limit_M_eq_orig)
+  show "B t \<subseteq> snap_actions"
+  proof (rule subsetI)
+    fix x
+    assume "x \<in> B t"
+    then have "\<exists>a. (x = at_start a \<or> x = at_end a) \<and> a \<in> actions" 
+      unfolding happ_at_def plan_happ_seq_def using plan_actions_in_problem
+      by blast
+    then show "x \<in> snap_actions" unfolding snap_actions_def by blast
+  qed
+qed
+
+lemma exec_time_full_upd_eq_exec_time': "partial_exec_time_update a t M = exec_time' a t"
+  using partial_exec_time_update_def exec_time_def exec_time'_def 
+    a_not_in_b_last_unchanged a_in_b_last_now B_lim_M_eq_B 
+  by simp
+
+lemma updated_exec_time_and_next: "exec_time a (t (Suc l)) = (exec_time' a (t l)) + (t (Suc l) - t l)"
+
+
+definition "W\<^sub>0 \<equiv> \<lambda>c. 0"
+
+lemma automaton_complete: "\<exists>W'. \<T> \<turnstile> \<langle>Init, W\<^sub>0\<rangle> \<rightarrow>* \<langle>Goal, W'\<rangle>"
+  sorry
 end
 
 end
